

1.CO2	Convert the following function to its corresponding canonical POS form using boolean algebraic formulas: $F(a,b,c,d) = (a+b+c'd')(b+d)$
2.CO2	Simplify the following function: $((A.B)' + (C'+D')')' . ((A.B') + (C.(D+A'.D))) + A'C$

Question 1 Solution

$$\begin{aligned}
&F(a,b,c,d) \\
&= (a+b+c'd')(b+d) \\
&= (a+b+c')(a+b+d')(b+d) \\
&= (a+b+c'+d')(a+b+c'+d)(a+b+d'+c')(a+b+d'+c)(b+d+a')(b+d+a) \\
&= (a+b+c'+d')(a+b+c'+d)(a+b+d'+c')(a+b+d'+c)(b+d+a'+c')(b+d+a'+c)(b+d+a+c')(b+d+a+c) \\
&= (a+b+c'+d')(a+b+c'+d)(a+b+c'+d')(a+b+c+d')(a'+b+c'+d)(a'+b+c+d)(a+b+c'+d)(a+b+c+d) \\
&= (a+b+c'+d')(a+b+c'+d)(a+b+c+d')(a'+b+c'+d)(a'+b+c+d)(a+b+c+d) \\
&= \prod (3, 2, 1, 10, 8, 0) \\
&= \prod (0, 1, 2, 3, 8, 10)
\end{aligned}$$

Question 2 Solution

$$\begin{aligned}
&((A.B)' + (C'+D')')' . ((A.B') + (C.(D+A'.D))) + A'C \\
&= ((AB)')' ((C'+D')')' (AB'+CD+A'CD) + A'C \\
&= AB (C'+D') (AB'+CD (1+D')) + A'C \\
&= (ABC'+ABD') (AB'+CD) + A'C \\
&= ABC'AB' + ABC'CD + ABD'AB' + ABD'CD + A'C \\
&= 0 + 0 + 0 + 0 + A'C \\
&= A'C
\end{aligned}$$

1.CO2	Convert the following function to its corresponding canonical POS form using boolean algebraic formulas: $F(w,x,y,z) = (w+x+y'z')(x+z)$
2.CO2	Simplify the following function: $W'X+((W.X)'+(Y'+Z'))'.((W.X')+(Y.(Z+W'.Z)))$

Question 1 Solution

$$\begin{aligned}
F(w,x, y, z) &= (w+y'z'+x)(z+x) \\
&= (w+x+y')(w+x+z')(x+z) \\
&= (w+x+y'+z')(w+x+y'+z)(w+x+z'+y')(w+x+z'+y)(x+z+w')(x+z+w) \\
&= (w+x+y'+z')(w+x+y'+z)(w+x+z'+y')(w+x+z'+y)(x+z+w'+y')(x+z+w'+y)(x+z+w+y')(x+z+w+y) \\
&= (w+x+y'+z')(w+x+y'+z)(w+x+y'+z')(w+x+y+z')(w'+x+y'+z)(w'+x+y+z)(w+x+y'+z)(w+x+y+z) \\
&= (w+x+y'+z')(w+x+y'+z)(w+x+y+z')(w'+x+y'+z)(w'+x+y+z)(w+x+y+z) \\
&= \prod (3, 2, 1, 10, 8, 0) \\
&= \prod (0, 1, 2, 3, 8, 10)
\end{aligned}$$

Question 2 Solution

$$\begin{aligned}
&W'X+((W.X)'+(Y'+Z'))'.((W.X')+(Y.(Z+W'.Z))) \\
&= W'X+((WX)')' ((Y'+Z'))' (WX'+YZ+W'YZ) \\
&= W'X+WX (Y'+Z') (WX'+YZ (1+Z')) \\
&= W'X+(WXY'+WXZ') (WX'+YZ) \\
&= W'X+WXY'WX' + WXY'YZ + WXZ'WX' + WXZ'YZ \\
&= W'X+0 + 0 + 0 + 0 \\
&= W'X
\end{aligned}$$

1.CO2	Convert the following function to its corresponding canonical POS form using boolean algebraic formulas: $F(a,b, c, d) = (a'+b+c'd)(b'+d)$
2.CO2	Simplify the following function: $A'B+(A'+B'(A(B.B'))+(A'(C.C')))(C'+1)+AB'C'+B'C(B'+B)$

Question 1 Solution

$$\begin{aligned}
F(a,b, c, d) &= (a'+b+c'd)(b'+d) \\
&= (a'+b+c')(a'+b+d)(b'+d) \\
&= (a'+b+c'+dd')(a'+b+cc'+d)(aa'+b'+d) \\
&= (a'+b+c'+d)(a'+b+c'+d')(a'+b+c+d)(a'+b+c'+d)(a+b'+d)(a'+b'+d) \\
&= (a'+b+c'+d)(a'+b+c'+d')(a'+b+c+d)(a'+b+c'+d)(a+b'+cc'+d)(a'+b'+cc'+d) \\
&= (a'+b+c'+d)(a'+b+c'+d')(a'+b+c+d)(a'+b+c'+d)(a+b'+c+d)(a+b'+c'+d)(a'+b'+c+d)(a'+b'+c'+d) \\
&= (1010)(1011)(1000)(1010)(0100)(0110)(1100)(1110) \\
&= \prod (10,11,8,10,4,6,12,14) \\
&= \prod (4,6,8,10,11,12,14)
\end{aligned}$$

Question 2 Solution

$$\begin{aligned}
&A'B+(A'+B'(A(B.B'))+(A'(C.C')))(C'+1)+AB'C'+B'C(B'+B) \\
&= A'B + (A'+0) + (0) (1) + AB'C'+B'C(1) \\
&= A'B + A' + AB'C' + B'C \\
&= A' (B+1) + B' (AC'+C) \\
&= A' + B' (A+C) (C'+C) \\
&= A' + B' (A+C) (1) \\
&= A' + B' (A+C) \\
&= A' + AB' + B'C \\
&= (A'+A) (A'+B') + B'C \\
&= A'+B'+B'C \\
&= A'+B'(1+C) \\
&= A'+B'
\end{aligned}$$

1.CO2	Convert the following function to its corresponding canonical POS form using boolean algebraic formulas: $F(w,x, y, z) = (w'+x+y'z)(x'+z)$
2.CO2	Simplify the following function: $P'Q+(P'+Q'(P(Q.Q'))+(P'(R.R')))(R'+1)+PQ'R'+Q'R(Q'+Q)$

Question 1 Solution

$$\begin{aligned}
F(w,x, y, z) &= (w'+x+y'z)(x'+z) \\
&= (w'+x+y')(w'+x+z)(x'+z) \\
&= (w'+x+y'+zz')(w'+x+yy'+z)(ww'+x'+z) \\
&= (w'+x+y'+z)(w'+x+y'+z')(w'+x+y+z)(w'+x+y'+z)(w+x'+z)(w'+x'+z) \\
&= (w'+x+y'+z)(w'+x+y'+z')(w'+x+y+z)(w'+x+y'+z)(w+x'+yy'+z)(w'+x'+yy'+z) \\
&= (w'+x+y'+z)(w'+x+y'+z')(w'+x+y+z)(w'+x+y'+z)(w+x'+y+z)(w+x'+y'+z)(w'+x'+y+z)(w'+x'+y'+z) \\
&= (1010)(1011)(1000)(1010)(0100)(0110)(1100)(1110) \\
&= \prod (10,11,8,10,4,6,12,14) \\
&= \prod (4,6,8,10,11,12,14)
\end{aligned}$$

Question 2 Solution

$$\begin{aligned}
&P'Q+(P'+Q'(P(Q.Q'))+(P'(R.R')))(R'+1)+PQ'R'+Q'R(Q'+Q) \\
&= P'Q+(P'+Q'(P(Q.Q'))+(P'(R.R')))(R'+1)+PQ'R'+Q'R(Q'+Q) \\
&= P'Q + (P'+0) + (0) (1) + PQ'R'+Q'R(1) \\
&= P'Q + P' + PQ'R' + Q'R \\
&= P' (Q+1) + Q' (PR'+R) \\
&= P' + Q' (P+R) (R'+R) \\
&= P' + Q' (P+R) (1) \\
&= P' + Q' (P+R) \\
&= P'+ PQ' + Q'R \\
&= (P'+P) (P'+Q') + Q'R \\
&= P'+Q'+Q'R \\
&= P'+Q'(1+R) \\
&= P'+Q'
\end{aligned}$$